tla-tree/MissingLibrary.dfy
@@ -67,3 +67,4 @@ function {:opaque} MemsetSeq<V>(v:V, len:nat) : (s:seq<V>)
 }
 
 } // module
+
